two schema entries
Signed-off-by: Shaobo He <shaobohe@amazon.com>

cedar-lean/Cedar/Validation/Types.lean
@@ -61,10 +61,34 @@ abbrev QualifiedType := Qualified CedarType
 
 abbrev RecordType := Map Attr QualifiedType
 
-structure EntitySchemaEntry where
+structure StandardSchemaEntry where
   ancestors : Cedar.Data.Set EntityType
   attrs : RecordType
   tags : Option CedarType
+
+inductive EntitySchemaEntry where
+  | standard (ty: StandardSchemaEntry)
+  | enum (eids: List String)
+
+def EntitySchemaEntry.validEid? (entry: EntitySchemaEntry) (eid: String): Bool :=
+  match entry with
+  | .standard _ => true
+  | .enum eids => eids.contains eid
+
+def EntitySchemaEntry.tags (entry: EntitySchemaEntry): Option CedarType :=
+  match entry with
+  | .standard ty => ty.tags
+  | .enum _ => none
+
+def EntitySchemaEntry.attrs (entry: EntitySchemaEntry): RecordType :=
+  match entry with
+  | .standard ty => ty.attrs
+  | .enum _ => Map.empty
+
+def EntitySchemaEntry.ancestors (entry: EntitySchemaEntry): Set EntityType :=
+  match entry with
+  | .standard ty => ty.ancestors
+  | .enum _ => Set.empty
 
 abbrev EntitySchema := Map EntityType EntitySchemaEntry
 
@@ -72,10 +96,16 @@ def EntitySchema.contains (ets : EntitySchema) (ety : EntityType) : Bool :=
   (ets.find? ety).isSome
 
 def EntitySchema.attrs? (ets : EntitySchema) (ety : EntityType) : Option RecordType :=
-  (ets.find? ety).map EntitySchemaEntry.attrs
+  (ets.find? ety).map λ e =>
+  match e with
+  | .standard ty => ty.attrs
+  | .enum _ => Map.empty
 
 def EntitySchema.tags? (ets : EntitySchema) (ety : EntityType) : Option (Option CedarType) :=
-  (ets.find? ety).map EntitySchemaEntry.tags
+  (ets.find? ety).map λ e =>
+  match e with
+  | .standard ty => ty.tags
+  | .enum _ => none
 
 def EntitySchema.descendentOf (ets : EntitySchema) (ety₁ ety₂ : EntityType) : Bool :=
   if ety₁ = ety₂
@@ -124,8 +154,8 @@ deriving instance Repr, DecidableEq, Inhabited for ExtType
 deriving instance Repr, DecidableEq, Inhabited for Qualified
 deriving instance Repr, Inhabited for CedarType
 deriving instance Repr for ActionSchemaEntry
-deriving instance Repr for EntitySchemaEntry
-deriving instance Repr for Schema
+-- deriving instance Repr for EntitySchemaEntry
+--deriving instance Repr for Schema
 
 mutual
 
