cedar-lean/Cedar/Thm/Validation/Typechecker/BinaryApp.lean
@@ -903,7 +903,10 @@ private theorem no_tags_type_implies_no_tags {uid : EntityUID} {env : Environmen
     replace ⟨e', h₂, h₃⟩ := h₂
     simp only [hf', Option.some.injEq] at h₂
     subst h₂
-    simp only [h₃] at h₁
+    simp only [EntitySchemaEntry.tags] at h₁
+    split at h₃
+    · simp only [h₃] at h₁
+      simp only [h₁, map_empty_contains_instance_of_ff]
     simp only [h₁, map_empty_contains_instance_of_ff]
   · exact map_empty_contains_instance_of_ff
 
@@ -1071,6 +1074,8 @@ theorem type_of_getTag_is_sound {x₁ x₂ : Expr} {c₁ c₂ : Capabilities} {e
   replace ⟨_, h₅, h₇⟩ := h₅
   simp only [hf₂, Option.some.injEq] at h₅
   subst h₅
+  simp only [EntitySchemaEntry.tags] at h₂
+  split at h₇
   simp only [h₇] at h₂
   have hf₃ := Map.findOrErr_returns d.tags s Error.tagDoesNotExist
   rcases hf₃ with ⟨v, hf₃⟩ | hf₃ <;>
@@ -1085,6 +1090,7 @@ theorem type_of_getTag_is_sound {x₁ x₂ : Expr} {c₁ c₂ : Capabilities} {e
     simp only [Entities.tagsOrEmpty, hf₁, Map.contains_iff_some_find?] at h₁
     replace ⟨_, h₁⟩ := h₁
     simp only [Map.findOrErr_err_iff_find?_none, h₁, reduceCtorEq] at hf₃
+  · cases h₇
 
 theorem type_of_binaryApp_is_sound {op₂ : BinaryOp} {x₁ x₂ : Expr} {c₁ c₂ : Capabilities} {env : Environment} {ty : TypedExpr} {request : Request} {entities : Entities}
   (h₁ : CapabilitiesInvariant c₁ request entities)
